interface/Set_extended.fst
@@ -11,9 +11,10 @@ let mem #a x s = s x
 let equal #a s1 s2 = F.feq s1 s2
 let union #a s1 s2 = F.on_dom a (fun x -> s1 x || s2 x)
 let intersection #a s1 s2 = F.on_dom a (fun x -> s1 x && s2 x)
+let complement #a s = F.on_dom a (fun x -> not (s x))
 let difference #a s1 s2 = F.on_dom a (fun x -> s1 x && not (s2 x))
 let filter #a s1 p = F.on_dom a (fun x -> s1 x && p x)
-//let remove #a s1 x = F.on_dom a (fun y -> s1 y && x <> y)
+let remove #a s1 x = F.on_dom a (fun y -> s1 y && x <> y)
 
 let mem_empty #a x = ()
 let equal_intro #a s1 s2 = ()
@@ -25,8 +26,9 @@ let subset_mem #a s1 s2 = ()
 let mem_union #a s1 s2 x = ()
 let mem_singleton #a x y = ()
 let mem_intersection #a s1 s2 x = ()
+let mem_complement #a s x = ()
 let mem_difference #a s1 s2 x = ()
 let mem_filter #a s p x = ()
-//let mem_remove_x #a s x = ()
-//let mem_remove_y #a s x y = ()
+let mem_remove_x #a s x = ()
+let mem_remove_y #a s x y = ()
           
