mrdts-new/Map/App_new.fst
@@ -1,267 +1,266 @@
 module App_new
 
-open FStar.Seq
+module M = Map_extended
+module S = Set_extended
 
 #set-options "--query_stats"
 
 // the concrete state type
-val concrete_st : Type0
+type concrete_st = S.t (pos & (nat & nat)) //set of (timestamp, (key, value))
 
 // init state
-val init_st : concrete_st
-
+let init_st : concrete_st = S.empty
+  
 // equivalence between 2 concrete states
-val eq (a b:concrete_st) : Type0
+let eq (a b:concrete_st) = S.equal a b
 
-val symmetric (a b:concrete_st) 
+let symmetric (a b:concrete_st) 
   : Lemma (requires eq a b)
-          (ensures eq b a)
+          (ensures eq b a) = ()
 
-val transitive (a b c:concrete_st)
+let transitive (a b c:concrete_st)
   : Lemma (requires eq a b /\ eq b c)
-          (ensures eq a c)
+          (ensures eq a c) = ()
 
-val eq_is_equiv (a b:concrete_st)
+let eq_is_equiv (a b:concrete_st)
   : Lemma (requires a == b)
-          (ensures eq a b)
+          (ensures eq a b) = ()
 
 // operation type
-val app_op_t : eqtype
+type app_op_t:eqtype =
+  |Set : nat -> nat -> app_op_t //key-value pair
+  |Del : nat -> app_op_t //key
 
-type op_t = pos (*timestamp*) & (nat (*replica ID*) & app_op_t)
-
-let get_rid (_,(rid,_)) = rid
-
-let distinct_ops (op1 op2:op_t) = fst op1 =!= fst op2
-
-type log = seq op_t
-
-// apply an operation to a state
-val do (s:concrete_st) (o:op_t) : concrete_st
-
-let commutes_with (o1 o2:op_t) =
-  forall s. eq (do (do s o1) o2) (do (do s o2) o1)
+let get_key (o:op_t) : nat =
+  match snd (snd o) with
+  |Set k v -> k
+  |Del k -> k
   
-// applying a log of operations to a concrete state
-let rec apply_log (x:concrete_st) (l:log) : Tot concrete_st (decreases length l) =
-  match length l with
-  |0 -> x
-  |_ -> apply_log (do x (head l)) (tail l)  
-
-// property of apply_log
-let rec lem_apply_log (x:concrete_st) (l:log)
-  : Lemma (requires true)
-          (ensures (length l > 0 ==> apply_log x l == do (apply_log x (fst (un_snoc l))) (last l)))
-          (decreases length l) =
-  match length l with
-  |0 -> ()
-  |_ -> lem_apply_log (do x (head l)) (tail l)
- 
-type rc_res =
-  |Fst_then_snd //o1 -> o2
-  |Snd_then_fst //o2 -> o1
-  |Either
+// apply an operation to a state
+let do (s:concrete_st) (o:op_t) : concrete_st =
+  match o with
+  |(ts, (_, Set k v)) -> S.add (ts, (k,v)) s 
+  |(_, (_, Del k)) -> S.filter s (fun e -> fst (snd e) <> k)
 
 //conflict resolution
-val rc (o1 o2:op_t) : rc_res
+let rc (o1 o2:op_t) =
+  match snd (snd o1), snd (snd o2) with
+  |Set k1 v2, Del k2 -> if k1 = k2 then Snd_then_fst else Either 
+  |Del k1, Set k2 v2 -> if k1 = k2 then Fst_then_snd else Either
+  |_ -> Either
 
 // concrete merge operation
-val merge (l a b:concrete_st) : concrete_st
+let merge (l a b:concrete_st) : concrete_st =
+  let da = S.difference a l in    //a - l
+  let db = S.difference b l in    //b - l
+  let i_ab = S.intersection a b in
+  let i_lab = S.intersection l i_ab in   // intersect l a b
+  S.union i_lab (S.union da db) 
 
 /////////////////////////////////////////////////////////////////////////////
+      
+let no_rc_chain (o1 o2 o3:op_t)  : Lemma (requires distinct_ops o1 o2 /\ distinct_ops o2 o3)
+          (ensures ~ (Fst_then_snd? (rc o1 o2) /\ Fst_then_snd? (rc o2 o3))) = ()
 
-val no_rc_chain (o1 o2 o3:op_t)
-  : Lemma (requires distinct_ops o1 o2 /\ distinct_ops o2 o3)
-          (ensures ~ (Fst_then_snd? (rc o1 o2) /\ Fst_then_snd? (rc o2 o3)))
-
-val relaxed_comm (s:concrete_st) (o1 o2 o3:op_t)
+let relaxed_comm (s:concrete_st) (o1 o2 o3:op_t)
   : Lemma (requires distinct_ops o1 o2 /\ distinct_ops o2 o3 /\ Fst_then_snd? (rc o1 o2) /\ ~ (Either? (rc o2 o3)))
-          (ensures eq (do (do (do s o1) o2) o3) (do (do (do s o2) o1) o3))
+          (ensures eq (do (do (do s o1) o2) o3) (do (do (do s o2) o1) o3)) = ()
 
-val non_comm (o1 o2:op_t)
+let non_comm (o1 o2:op_t)
   : Lemma (requires distinct_ops o1 o2)
-          (ensures Either? (rc o1 o2) <==> commutes_with o1 o2)
+          (ensures Either? (rc o1 o2) <==> commutes_with o1 o2) =
+   assert (((Set? (snd (snd o1)) /\ Del? (snd (snd o2)) /\ get_key o1 = get_key o2) \/ 
+           (Del? (snd (snd o1)) /\ Set? (snd (snd o2)) /\ get_key o1 = get_key o2)) ==>
+           ~ (eq (do (do init_st o1) o2) (do (do init_st o2) o1))); ()
 
-val cond_comm (o1:op_t) (o2:op_t{distinct_ops o1 o2 /\ ~ (Either? (rc o1 o2))}) (o3:op_t) : bool
+let cond_comm (o1:op_t) (o2:op_t{distinct_ops o1 o2 /\ ~ (Either? (rc o1 o2))}) (o3:op_t)=
+  if Del? (snd (snd o3)) && get_key o1 = get_key o3 then true else false
 
-val cond_comm_base (s:concrete_st) (o1 o2 o3:op_t)
+#push-options "--z3rlimit 50 --max_ifuel 3 --split_queries on_failure"
+let cond_comm_base (s:concrete_st) (o1 o2 o3:op_t)
   : Lemma (requires distinct_ops o1 o2 /\ ~ (Either? (rc o1 o2)) /\ cond_comm o1 o2 o3)
-          (ensures eq (do (do (do s o1) o2) o3) (do (do (do s o2) o1) o3))
+          (ensures eq (do (do (do s o1) o2) o3) (do (do (do s o2) o1) o3)) = ()
 
-val cond_comm_ind (s:concrete_st) (o1 o2 o3 o:op_t) (l:log)
+let cond_comm_ind (s:concrete_st) (o1 o2 o3 o:op_t) (l:log)
   : Lemma (requires distinct_ops o1 o2 /\ ~ (Either? (rc o1 o2)) /\ cond_comm o1 o2 o3 /\
                     eq (do (apply_log (do (do s o1) o2) l) o3) (do (apply_log (do (do s o2) o1) l) o3))
-          (ensures eq (do (do (apply_log (do (do s o1) o2) l) o) o3) (do (do (apply_log (do (do s o2) o1) l) o) o3))
-                  
-////////////////////////////////////////////////////////////////////////////
+          (ensures eq (do (do (apply_log (do (do s o1) o2) l) o) o3) (do (do (apply_log (do (do s o2) o1) l) o) o3)) = ()
+  
+/////////////////////////////////////////////////////////////////////////////
+// Merge commutativity
+let merge_comm (l a b:concrete_st)
+   : Lemma (ensures (eq (merge l a b) (merge l b a))) = ()
 
-val merge_comm (l a b:concrete_st)
-  : Lemma (ensures (eq (merge l a b) (merge l b a)))
-                       
-val merge_idem (s:concrete_st)
-  : Lemma (ensures eq (merge s s s) s)
+// Merge idempotence
+let merge_idem (s:concrete_st)
+   : Lemma (ensures eq (merge s s s) s) = ()
 
 (*Two OP RC*)
 //////////////// 
-val rc_ind_right (l a b:concrete_st) (o1 o2' o2:op_t)
-  : Lemma (requires distinct_ops o1 o2 /\ Fst_then_snd? (rc o1 o2) /\
-                    eq (merge l (do a o1) (do b o2)) (do (merge l (do a o1) b) o2))
-          (ensures eq (merge l (do a o1) (do (do b o2') o2)) (do (merge l (do a o1) (do b o2')) o2))
+let rc_ind_right (l a b:concrete_st) (o1 o2' o2:op_t)
+   : Lemma (requires distinct_ops o1 o2 /\ Fst_then_snd? (rc o1 o2) /\
+                     eq (merge l (do a o1) (do b o2)) (do (merge l (do a o1) b) o2))
+           (ensures eq (merge l (do a o1) (do (do b o2') o2)) (do (merge l (do a o1) (do b o2')) o2)) = ()
 
-val rc_ind_left (l a b:concrete_st) (o1 o1' o2:op_t)
+let rc_ind_left (l a b:concrete_st) (o1 o1' o2:op_t)
   : Lemma (requires distinct_ops o1 o2 /\ Fst_then_snd? (rc o1 o2) /\
                     eq (merge l (do a o1) (do b o2)) (do (merge l (do a o1) b) o2))
-          (ensures eq (merge l (do (do a o1') o1) (do b o2)) (do (merge l (do (do a o1') o1) b) o2))
+          (ensures eq (merge l (do (do a o1') o1) (do b o2)) (do (merge l (do (do a o1') o1) b) o2)) = ()
+
 //Special case of rc_intermediate_v1
-val rc_base (l:concrete_st) (o o1 o2:op_t)
+let rc_base (l:concrete_st) (o o1 o2:op_t)
   : Lemma (requires distinct_ops o1 o2 /\ Fst_then_snd? (rc o1 o2) /\ distinct_ops o o1 /\ distinct_ops o o2 /\
                     eq (merge l (do l o1) (do l o2)) (do (do l o1) o2))
-          (ensures eq (merge (do l o) (do (do l o) o1) (do (do l o) o2)) (do (do (do l o) o1) o2))
-
-val rc_base_base (o1 o2:op_t)
+          (ensures eq (merge (do l o) (do (do l o) o1) (do (do l o) o2)) (do (do (do l o) o1) o2)) = ()
+          
+let rc_base_base (o1 o2:op_t)
   : Lemma (requires distinct_ops o1 o2 /\ Fst_then_snd? (rc o1 o2))
-          (ensures eq (merge init_st (do init_st o1) (do init_st o2)) (do (do init_st o1) o2))
+          (ensures eq (merge init_st (do init_st o1) (do init_st o2)) (do (do init_st o1) o2)) = 
+  let lhs = (merge init_st (do init_st o1) (do init_st o2)) in
+  let rhs = (do (do init_st o1) o2) in
+  //assert (forall k. M.contains lhs k = M.contains rhs k);
+  ()
 
-val rc_intermediate_base_right (l s1 s2 s3:concrete_st) (o o' o1 o2:op_t) 
+let rc_intermediate_base_right (l s1 s2 s3:concrete_st) (o o' o1 o2:op_t) 
   : Lemma (requires distinct_ops o o' /\ Fst_then_snd? (rc o o') /\ 
                     distinct_ops o1 o2 /\ Fst_then_snd? (rc o1 o2) /\
                     eq (merge (do l o') (do (do s1 o') o1) (do (do s2 o') o2)) (do (do (do s3 o') o1) o2) /\
                     eq (merge l (do s1 o1) (do s2 o2)) (do (do s3 o1) o2) /\
                     eq (merge l (do s1 o') (do s2 o)) (do (do s3 o) o')) //***EXTRA***
-          (ensures eq (merge (do l o') (do (do s1 o') o1) (do (do (do s2 o) o') o2)) (do (do (do (do s3 o) o') o1) o2))
-
-val rc_intermediate_base_left_right (l s1 s2 s3:concrete_st) (o o' o1' o1 o2:op_t) 
+          (ensures eq (merge (do l o') (do (do s1 o') o1) (do (do (do s2 o) o') o2)) (do (do (do (do s3 o) o') o1) o2)) = ()
+          
+let rc_intermediate_base_left_right (l s1 s2 s3:concrete_st) (o o' o1' o1 o2:op_t) 
   : Lemma (requires distinct_ops o o' /\ Fst_then_snd? (rc o o') /\  
                     distinct_ops o1 o2 /\ Fst_then_snd? (rc o1 o2) /\
                     distinct_ops o1' o' /\ Fst_then_snd? (rc o1' o') /\
                     eq (merge (do l o') (do (do s1 o') o1) (do (do s2 o') o2)) (do (do (do s3 o') o1) o2) /\
                     eq (merge l (do s1 o1) (do s2 o2)) (do (do s3 o1) o2)) 
-        (ensures eq (merge (do l o') (do (do (do s1 o1') o') o1) (do (do (do s2 o) o') o2)) (do (do (do (do (do s3 o1') o) o') o1) o2))
+        (ensures eq (merge (do l o') (do (do (do s1 o1') o') o1) (do (do (do s2 o) o') o2)) (do (do (do (do (do s3 o1') o) o') o1) o2)) = ()
 
-val rc_intermediate_2_right (l s1 s2 s3:concrete_st) (o1 o2 o o':op_t) (o_n:op_t{~ (commutes_with o_n o)})
+let rc_intermediate_2_right (l s1 s2 s3:concrete_st) (o1 o2 o o':op_t) (o_n:op_t{~ (commutes_with o_n o)})
   : Lemma (requires distinct_ops o1 o2 /\ Fst_then_snd? (rc o1 o2) /\  
                     distinct_ops o o' /\ Fst_then_snd? (rc o o') /\
                     get_rid o_n <> get_rid o' (*o_n,o' must be concurrent*) /\
                     eq (merge (do l o') (do (do s1 o') o1) (do (do (do s2 o) o') o2)) (do (do (do (do s3 o) o') o1) o2))
-      (ensures eq (merge (do l o') (do (do s1 o') o1) (do (do (do (do s2 o_n) o) o') o2)) (do (do (do (do (do s3 o_n) o) o') o1) o2)) 
+          (ensures eq (merge (do l o') (do (do s1 o') o1) (do (do (do (do s2 o_n) o) o') o2)) (do (do (do (do (do s3 o_n) o) o') o1) o2)) = ()
 
-val rc_intermediate_2_left (l s1 s2 s3:concrete_st) (o1 o2:op_t) (o o':op_t) (o_n:op_t{~ (commutes_with o_n o)})
+let rc_intermediate_2_left (l s1 s2 s3:concrete_st) (o1 o2 o o':op_t) (o_n:op_t{~ (commutes_with o_n o)})
   : Lemma (requires distinct_ops o1 o2 /\ Fst_then_snd? (rc o1 o2) /\  
                     distinct_ops o o' /\ Fst_then_snd? (rc o o') /\
                     get_rid o_n <> get_rid o' (*o_n,o' must be concurrent*) /\
                     eq (merge (do l o') (do (do (do s1 o) o') o1) (do (do s2 o') o2)) (do (do (do (do s3 o) o') o1) o2))
-      (ensures eq (merge (do l o') (do (do (do (do s1 o_n) o) o') o1) (do (do s2 o') o2)) (do (do (do (do (do s3 o_n) o) o') o1) o2))
+          (ensures eq (merge (do l o') (do (do (do (do s1 o_n) o) o') o1) (do (do s2 o') o2)) (do (do (do (do (do s3 o_n) o) o') o1) o2)) = ()
 
 // In general, the events o',o_n, below should be such that these exists o, (rc o o')
-val rc_intermediate_1_v2 (l s1 s2 s3:concrete_st) (o1 o2 o' o_n:op_t)
+let rc_intermediate_1_v2 (l s1 s2 s3:concrete_st) (o1 o2 o' o_n:op_t)
   : Lemma (requires distinct_ops o1 o2 /\ Fst_then_snd? (rc o1 o2) /\ 
                     (exists o. Fst_then_snd? (rc o o')) /\ (exists o. Fst_then_snd? (rc o o_n)) /\ 
                     eq (merge (do l o_n) (do (do s1 o_n) o1) (do (do s2 o_n) o2)) (do (do (do s3 o_n) o1) o2) /\
                     eq (merge (do l o') (do (do s1 o') o1) (do (do s2 o') o2)) (do (do (do s3 o') o1) o2))
-    (ensures eq (merge (do (do l o_n) o') (do (do (do s1 o_n) o') o1) (do (do (do s2 o_n) o') o2)) (do (do (do (do s3 o_n) o') o1) o2))
+    (ensures eq (merge (do (do l o_n) o') (do (do (do s1 o_n) o') o1) (do (do (do s2 o_n) o') o2)) (do (do (do (do s3 o_n) o') o1) o2)) = ()
 
 (*One op*)
 ///////////////
-val ind_right_one_op (l a b c:concrete_st) (o1 o1':op_t)
+let ind_right_one_op (l a b c:concrete_st) (o1 o1':op_t)
    : Lemma (requires eq (merge l a (do b o1)) (do (merge l a b) o1))
-           (ensures eq (merge l a (do (do b o1') o1)) (do (merge l a (do b o1')) o1))
+           (ensures eq (merge l a (do (do b o1') o1)) (do (merge l a (do b o1')) o1)) = ()
            
-val base_one_op (l:concrete_st) (o o1:op_t)
+let base_one_op (l:concrete_st) (o o1:op_t)
   : Lemma (requires eq (merge l l (do l o1)) (do l o1))
-          (ensures eq (merge (do l o) (do l o) (do (do l o) o1)) (do (do l o) o1)) 
+          (ensures eq (merge (do l o) (do l o) (do (do l o) o1)) (do (do l o) o1)) = ()
 
-val base_base_one_op (o1:op_t)
-  : Lemma (ensures eq (merge init_st init_st (do init_st o1)) (do init_st o1))
+let base_base_one_op (o1:op_t)
+  : Lemma (ensures eq (merge init_st init_st (do init_st o1)) (do init_st o1)) = ()
 
-val intermediate_base_right_one_op (l s1 s2 s3:concrete_st) (o o' o1:op_t) 
+let intermediate_base_right_one_op (l s1 s2 s3:concrete_st) (o o' o1:op_t) 
   : Lemma (requires distinct_ops o o' /\ Fst_then_snd? (rc o o') /\
                     eq (merge (do l o') (do s1 o') (do (do s2 o') o1)) (do (do s3 o') o1) /\
                     eq (merge l s1 (do s2 o1)) (do s3 o1) /\
                     eq (merge l (do s1 o') (do s2 o)) (do (do s3 o) o')) //***EXTRA***
-          (ensures eq (merge (do l o') (do s1 o') (do (do (do s2 o) o') o1)) (do (do (do s3 o) o') o1))
+          (ensures eq (merge (do l o') (do s1 o') (do (do (do s2 o) o') o1)) (do (do (do s3 o) o') o1)) = ()
 
-val intermediate_base_right_one_op_left (l s1 s2 s3:concrete_st) (o o' o1:op_t) 
+let intermediate_base_right_one_op_left (l s1 s2 s3:concrete_st) (o o' o1:op_t) 
   : Lemma (requires distinct_ops o o' /\ Fst_then_snd? (rc o o') /\ distinct_ops o' o1 /\
                     eq (merge (do l o') (do (do s1 o') o1) (do s2 o')) (do (do s3 o') o1) /\
                     (Fst_then_snd? (rc o o1) ==> eq (merge l (do s1 o1) (do s2 o)) (do (merge l s1 (do s2 o)) o1)) /\ //***EXTRA***       
                     eq (merge l (do s1 o1) s2) (do s3 o1) /\
                     eq (merge l (do s1 o') (do s2 o)) (do (do s3 o) o')) //***EXTRA***
-          (ensures eq (merge (do l o') (do (do s1 o') o1) (do (do s2 o) o')) (do (do (do s3 o) o') o1))
+          (ensures eq (merge (do l o') (do (do s1 o') o1) (do (do s2 o) o')) (do (do (do s3 o) o') o1)) = ()
 
-val intermediate_base_left_one_op (l s1 s2 s3:concrete_st) (o o' o1:op_t) 
+let intermediate_base_left_one_op (l s1 s2 s3:concrete_st) (o o' o1:op_t) 
   : Lemma (requires distinct_ops o o' /\ Fst_then_snd? (rc o o') /\
                     eq (merge (do l o') (do s1 o') (do (do s2 o') o1)) (do (do s3 o') o1) /\
                     (Fst_then_snd? (rc o o1) ==> eq (merge l (do s1 o1) (do s2 o)) (do (merge l s1 (do s2 o)) o1)) /\ //***EXTRA***
                     eq (merge l s1 (do s2 o1)) (do s3 o1) /\
                     eq (merge l (do s1 o') (do s2 o)) (do (do s3 o) o') /\ //***EXTRA***
                     eq (merge l (do (do s1 o) o') (do s2 o')) (do (do s3 o) o')) //***EXTRA***
-          (ensures eq (merge (do l o') (do (do s1 o) o') (do (do s2 o') o1)) (do (do (do s3 o) o') o1))
+          (ensures eq (merge (do l o') (do (do s1 o) o') (do (do s2 o') o1)) (do (do (do s3 o) o') o1)) = ()
 
-val intermediate_base_left_right_one_op (l s1 s2 s3:concrete_st) (o o' o1' o1:op_t) 
+let intermediate_base_left_right_one_op (l s1 s2 s3:concrete_st) (o o' o1' o1:op_t) 
   : Lemma (requires distinct_ops o o' /\ Fst_then_snd? (rc o o') /\
                     distinct_ops o1' o' /\ Fst_then_snd? (rc o1' o') /\
                     eq (merge (do l o') (do s1 o') (do (do s2 o') o1)) (do (do s3 o') o1) /\
                     eq (merge (do l o') (do (do s1 o1') o') (do (do s2 o') o1)) (do (do (do s3 o1') o') o1) /\ //EXTRA
                     eq (merge l s1 (do s2 o1)) (do s3 o1))
-          (ensures eq (merge (do l o') (do (do s1 o1') o') (do (do (do s2 o) o') o1)) (do (do (do (do s3 o1') o) o') o1))
+          (ensures eq (merge (do l o') (do (do s1 o1') o') (do (do (do s2 o) o') o1)) (do (do (do (do s3 o1') o) o') o1)) = ()
 
-val intermediate_2_left_one_op (l s1 s2 s3:concrete_st) (o1 o o':op_t) (o_n:op_t{~ (commutes_with o_n o)})
+let intermediate_2_left_one_op (l s1 s2 s3:concrete_st) (o1 o o':op_t) (o_n:op_t{~ (commutes_with o_n o)})
   : Lemma (requires distinct_ops o o' /\ Fst_then_snd? (rc o o') /\
                     get_rid o_n <> get_rid o' (*o_n,o' must be concurrent*) /\
                     eq (merge (do l o') (do (do s1 o) o') (do (do s2 o') o1)) (do (do (do s3 o) o') o1))
-          (ensures eq (merge (do l o') (do (do (do s1 o_n) o) o') (do (do s2 o') o1)) (do (do (do (do s3 o_n) o) o') o1))
+          (ensures eq (merge (do l o') (do (do (do s1 o_n) o) o') (do (do s2 o') o1)) (do (do (do (do s3 o_n) o) o') o1)) = ()
 
 // In general, the events o',o_n, below should be such that these exists o, (rc o o')
-val intermediate_1_v2_one_op (l s1 s2 s3:concrete_st) (o1 o' o_n:op_t)
+let intermediate_1_v2_one_op (l s1 s2 s3:concrete_st) (o1 o' o_n:op_t)
   : Lemma (requires (exists o. Fst_then_snd? (rc o o')) /\ (exists o. Fst_then_snd? (rc o o_n)) /\ 
                     eq (merge (do l o_n) (do s1 o_n) (do (do s2 o_n) o1)) (do (do s3 o_n) o1) /\
                     eq (merge (do l o') (do s1 o') (do (do s2 o') o1)) (do (do s3 o') o1))
-          (ensures eq (merge (do (do l o_n) o') (do (do s1 o_n) o') (do (do (do s2 o_n) o') o1)) (do (do (do s3 o_n) o') o1))
+          (ensures eq (merge (do (do l o_n) o') (do (do s1 o_n) o') (do (do (do s2 o_n) o') o1)) (do (do (do s3 o_n) o') o1)) = ()
 
 (*Zero op *)
 ///////////////
-val intermediate_base_right_zero_op (l s1 s2 s3:concrete_st) (o o':op_t) 
+let intermediate_base_right_zero_op (l s1 s2 s3:concrete_st) (o o':op_t) 
   : Lemma (requires distinct_ops o o' /\ Fst_then_snd? (rc o o') /\
                     eq (merge (do l o') (do s1 o') (do s2 o')) (do s3 o') /\
                     eq (merge l s1 s2) s3 /\
                     eq (merge l (do s1 o') (do s2 o)) (do (do s3 o) o')) //***EXTRA***
-          (ensures eq (merge (do l o') (do s1 o') (do (do s2 o) o')) (do (do s3 o) o')) 
+          (ensures eq (merge (do l o') (do s1 o') (do (do s2 o) o')) (do (do s3 o) o')) = ()
 
-val intermediate_base_left_right_zero_op (l s1 s2 s3:concrete_st) (o o' o1':op_t) 
+let intermediate_base_left_right_zero_op (l s1 s2 s3:concrete_st) (o o' o1':op_t) 
   : Lemma (requires distinct_ops o o' /\ Fst_then_snd? (rc o o') /\  
                     distinct_ops o1' o' /\ Fst_then_snd? (rc o1' o') /\
                     eq (merge (do l o') (do s1 o') (do s2 o')) (do s3 o') /\
                     eq (merge l s1 s2) s3) 
-          (ensures eq (merge (do l o') (do (do s1 o1') o') (do (do s2 o) o')) (do (do (do s3 o1') o) o'))
+          (ensures eq (merge (do l o') (do (do s1 o1') o') (do (do s2 o) o')) (do (do (do s3 o1') o) o')) = ()
 
-val intermediate_2_right_zero_op (l s1 s2 s3:concrete_st) (o o':op_t) (o_n:op_t{~ (commutes_with o_n o)})
+let intermediate_2_right_zero_op (l s1 s2 s3:concrete_st) (o o':op_t) (o_n:op_t{~ (commutes_with o_n o)})
   : Lemma (requires distinct_ops o o' /\ Fst_then_snd? (rc o o') /\
                     get_rid o_n <> get_rid o' (*o_n,o' must be concurrent*) /\
                     eq (merge (do l o') (do s1 o') (do (do s2 o) o')) (do (do s3 o) o'))
-          (ensures eq (merge (do l o') (do s1 o') (do (do (do s2 o_n) o) o')) (do (do (do s3 o_n) o) o')) 
+          (ensures eq (merge (do l o') (do s1 o') (do (do (do s2 o_n) o) o')) (do (do (do s3 o_n) o) o')) = ()
 
-val intermediate_2_left_zero_op (l s1 s2 s3:concrete_st) (o o':op_t) (o_n:op_t{~ (commutes_with o_n o)})
+let intermediate_2_left_zero_op (l s1 s2 s3:concrete_st) (o o':op_t) (o_n:op_t{~ (commutes_with o_n o)})
   : Lemma (requires distinct_ops o o' /\ Fst_then_snd? (rc o o') /\
                     get_rid o_n <> get_rid o' (*o_n,o' must be concurrent*) /\
                     eq (merge (do l o') (do (do s1 o) o') (do s2 o')) (do (do s3 o) o'))
-          (ensures eq (merge (do l o') (do (do (do s1 o_n) o) o') (do s2 o')) (do (do (do s3 o_n) o) o')) 
+          (ensures eq (merge (do l o') (do (do (do s1 o_n) o) o') (do s2 o')) (do (do (do s3 o_n) o) o')) = ()
 
 // In general, the event "o" below should be such that these exists o', (rc o' o)
-val intermediate_1_v1_zero_op (l s1 s2 s3:concrete_st) (o:op_t)
+let intermediate_1_v1_zero_op (l s1 s2 s3:concrete_st) (o:op_t)
   : Lemma (requires (exists o'. Fst_then_snd? (rc o' o)) /\ eq (merge l s1 s2) s3)
-          (ensures eq (merge (do l o) (do s1 o) (do s2 o)) (do s3 o))
+          (ensures eq (merge (do l o) (do s1 o) (do s2 o)) (do s3 o)) = ()
 
 // In general, the events o',o_n, below should be such that these exists o, (rc o o')
-val intermediate_1_v2_zero_op (l s1 s2 s3:concrete_st) (o' o_n:op_t)
+let intermediate_1_v2_zero_op (l s1 s2 s3:concrete_st) (o' o_n:op_t)
   : Lemma (requires (exists o. Fst_then_snd? (rc o o')) /\ (exists o. Fst_then_snd? (rc o o_n)) /\ 
                     eq (merge (do l o_n) (do s1 o_n) (do s2 o_n)) (do s3 o_n)  /\
                     eq (merge (do l o') (do s1 o') (do s2 o')) (do s3 o'))
-          (ensures eq (merge (do (do l o_n) o') (do (do s1 o_n) o') (do (do s2 o_n) o')) (do (do s3 o_n) o'))
+          (ensures eq (merge (do (do l o_n) o') (do (do s1 o_n) o') (do (do s2 o_n) o')) (do (do s3 o_n) o')) = ()
 
 (* 2 op Comm  *)
 ///////////////////
 
-val comm_ind_right (l a b c:concrete_st) (o1 o2' o2:op_t)
+let comm_ind_right (l a b c:concrete_st) (o1 o2' o2:op_t)
   : Lemma (requires distinct_ops o1 o2 /\ Either? (rc o1 o2) /\ distinct_ops o2' o1 /\
                     eq (merge l (do a o1) (do b o2)) (do (do (merge l a b) o2) o1) /\
                     (Fst_then_snd? (rc o2' o1) ==> (eq (merge l (do a o1) (do b o2')) (do (merge l a (do b o2')) o1))) /\
@@ -269,9 +268,9 @@ val comm_ind_right (l a b c:concrete_st) (o1 o2' o2:op_t)
                     ~ (Fst_then_snd? (rc o1 o2')) /\
                     ~ (exists o3 b'. eq (do (do b o2') o2) (do b' o3) /\ distinct_ops o1 o3 /\ Fst_then_snd? (rc o1 o3)) /\
                     ~ (exists o3 b'. eq (do b o2) (do b' o3) /\ distinct_ops o1 o3 /\ Fst_then_snd? (rc o1 o3)))                    
-          (ensures eq (merge l (do a o1) (do (do b o2') o2)) (do (do (merge l a (do b o2')) o2) o1))
+          (ensures eq (merge l (do a o1) (do (do b o2') o2)) (do (do (merge l a (do b o2')) o2) o1)) = ()
 
-val comm_ind_left (l a b c:concrete_st) (o1 o2' o2:op_t)
+let comm_ind_left (l a b c:concrete_st) (o1 o2' o2:op_t)
   : Lemma (requires distinct_ops o1 o2 /\ Either? (rc o1 o2) /\ distinct_ops o2' o2 /\
                     eq (merge l (do a o1) (do b o2)) (do (do (merge l a b) o2) o1) /\
                     (Fst_then_snd? (rc o2' o2) ==> (eq (merge l (do a o2') (do b o2)) (do (merge l (do a o2') b) o2))) /\
@@ -279,18 +278,18 @@ val comm_ind_left (l a b c:concrete_st) (o1 o2' o2:op_t)
                     ~ (Fst_then_snd? (rc o2 o2')) /\
                     ~ (exists o3 b'. eq (do (do b o2') o2) (do b' o3) /\ distinct_ops o1 o3 /\ Fst_then_snd? (rc o1 o3)) /\
                     ~ (exists o3 b'. eq (do b o2) (do b' o3) /\ distinct_ops o1 o3 /\ Fst_then_snd? (rc o1 o3)))                    
-          (ensures eq (merge l (do (do a o2') o1) (do b o2)) (do (do (merge l (do a o2') b) o2) o1))
+          (ensures eq (merge l (do (do a o2') o1) (do b o2)) (do (do (merge l (do a o2') b) o2) o1)) = ()
 
-val comm_base (l:concrete_st) (o o1 o2:op_t)
+let comm_base (l:concrete_st) (o o1 o2:op_t)
   : Lemma (requires distinct_ops o1 o2 /\ Either? (rc o1 o2) /\ distinct_ops o o1 /\ distinct_ops o o2 /\
                     eq (merge l (do l o1) (do l o2)) (do (do l o2) o1))
-          (ensures eq (merge (do l o) (do (do l o) o1) (do (do l o) o2)) (do (do (do l o) o2) o1))
+          (ensures eq (merge (do l o) (do (do l o) o1) (do (do l o) o2)) (do (do (do l o) o2) o1)) = ()
 
-val comm_base_base (o1 o2:op_t)
+let comm_base_base (o1 o2:op_t)
   : Lemma (requires distinct_ops o1 o2 /\ Either? (rc o1 o2))
-          (ensures eq (merge init_st (do init_st o1) (do init_st o2)) (do (do init_st o1) o2))
+          (ensures eq (merge init_st (do init_st o1) (do init_st o2)) (do (do init_st o1) o2)) = ()
 
-val comm_intermediate_base_right (l s1 s2 s3:concrete_st) (o o' o1 o2:op_t) 
+let comm_intermediate_base_right (l s1 s2 s3:concrete_st) (o o' o1 o2:op_t) 
   : Lemma (requires distinct_ops o o' /\ Fst_then_snd? (rc o o') /\ 
                     distinct_ops o1 o2 /\ Either? (rc o1 o2) /\
                     distinct_ops o' o1 /\ distinct_ops o' o2 /\
@@ -298,9 +297,9 @@ val comm_intermediate_base_right (l s1 s2 s3:concrete_st) (o o' o1 o2:op_t)
                     eq (merge (do l o') (do (do s1 o') o1) (do (do s2 o') o2)) (do (do (do s3 o') o1) o2) /\ 
                     eq (merge (do l o') (do s1 o') (do (do s2 o) o')) (do (do s3 o) o') /\ //comes from intermediate_base_zero_op
                     eq (merge l (do s1 o1) (do s2 o2)) (do (do s3 o1) o2)) 
-          (ensures eq (merge (do l o') (do (do s1 o') o1) (do (do (do s2 o) o') o2)) (do (do (do (do s3 o) o') o1) o2))
+          (ensures eq (merge (do l o') (do (do s1 o') o1) (do (do (do s2 o) o') o2)) (do (do (do (do s3 o) o') o1) o2)) = ()
 
-val comm_intermediate_base_left_right (l s1 s2 s3:concrete_st) (o o' o1' o1 o2:op_t) 
+let comm_intermediate_base_left_right (l s1 s2 s3:concrete_st) (o o' o1' o1 o2:op_t) 
   : Lemma (requires distinct_ops o o' /\ Fst_then_snd? (rc o o') /\ 
                     distinct_ops o1 o2 /\ Either? (rc o1 o2) /\
                     distinct_ops o1' o' /\ Fst_then_snd? (rc o1' o') /\
@@ -309,53 +308,26 @@ val comm_intermediate_base_left_right (l s1 s2 s3:concrete_st) (o o' o1' o1 o2:o
                     eq (merge l (do s1 o1) (do s2 o2)) (do (do s3 o1) o2) /\
                     eq (merge l (do (do s1 o1') o1) (do (do s2 o) o2)) (do (do (merge l (do s1 o1') (do s2 o)) o1) o2) /\ //comes from comm_ind_right
                     eq (merge (do l o') (do s1 o') (do (do s2 o) o')) (do (do s3 o) o')) //comes from intermediate_base_zero_op
-        (ensures eq (merge (do l o') (do (do (do s1 o1') o') o1) (do (do (do s2 o) o') o2)) (do (do (do (do (do s3 o1') o) o') o1) o2)) 
+        (ensures eq (merge (do l o') (do (do (do s1 o1') o') o1) (do (do (do s2 o) o') o2)) (do (do (do (do (do s3 o1') o) o') o1) o2)) = ()
 
-val comm_intermediate_2_right (l s1 s2 s3:concrete_st) (o1 o2 o o':op_t) (o_n:op_t{~ (commutes_with o_n o)})
+let comm_intermediate_2_right (l s1 s2 s3:concrete_st) (o1 o2 o o':op_t) (o_n:op_t{~ (commutes_with o_n o)})
   : Lemma (requires distinct_ops o1 o2 /\ Either? (rc o1 o2) /\  
                     distinct_ops o o' /\ Fst_then_snd? (rc o o') /\
                     get_rid o_n <> get_rid o' (*o_n,o' must be concurrent*) /\
                     distinct_ops o_n o' /\ Either? (rc o_n o') /\ 
                     eq (merge (do l o') (do (do s1 o') o1) (do (do (do s2 o) o') o2)) (do (do (do (do s3 o) o') o1) o2))
-          (ensures eq (merge (do l o') (do (do s1 o') o1) (do (do (do (do s2 o_n) o) o') o2)) (do (do (do (do (do s3 o_n) o) o') o1) o2))
+          (ensures eq (merge (do l o') (do (do s1 o') o1) (do (do (do (do s2 o_n) o) o') o2)) (do (do (do (do (do s3 o_n) o) o') o1) o2)) = ()
 
-val comm_intermediate_2_left (l s1 s2 s3:concrete_st) (o1 o2 o o':op_t) (o_n:op_t{~ (commutes_with o_n o)})
+let comm_intermediate_2_left (l s1 s2 s3:concrete_st) (o1 o2 o o':op_t) (o_n:op_t{~ (commutes_with o_n o)})
   : Lemma (requires distinct_ops o1 o2 /\ Either? (rc o1 o2) /\  
                     distinct_ops o o' /\ Fst_then_snd? (rc o o') /\
                     get_rid o_n <> get_rid o' (*o_n,o' must be concurrent*) /\
                     distinct_ops o_n o' /\ Either? (rc o_n o') /\ 
-                    //eq (merge (do l o') (do (do (do s1 o_n) o') o1) (do (do s2 o') o2)) (do (do (do (do s3 o_n) o') o1) o2) /\ //***EXTRA***
                     eq (merge (do l o') (do (do (do s1 o) o') o1) (do (do s2 o') o2)) (do (do (do (do s3 o) o') o1) o2))
-          (ensures eq (merge (do l o') (do (do (do (do s1 o_n) o) o') o1) (do (do s2 o') o2)) (do (do (do (do (do s3 o_n) o) o') o1) o2))
+          (ensures eq (merge (do l o') (do (do (do (do s1 o_n) o) o') o1) (do (do s2 o') o2)) (do (do (do (do (do s3 o_n) o) o') o1) o2)) = ()
 
-val comm_intermediate_1_v1 (l s1 s2 s3:concrete_st) (o1 o2 o:op_t)
+let comm_intermediate_1_v1 (l s1 s2 s3:concrete_st) (o1 o2 o:op_t)
   : Lemma (requires distinct_ops o1 o2 /\ Either? (rc o1 o2) /\ distinct_ops o1 o /\ distinct_ops o o2 /\
                     (exists o'. Fst_then_snd? (rc o' o)) /\
                     eq (merge l (do s1 o1) (do s2 o2)) (do (do s3 o1) o2))
-          (ensures eq (merge (do l o) (do (do s1 o) o1) (do (do s2 o) o2)) (do (do (do s3 o) o1) o2))
-
-////////////////////////////////////////////////////////////////
-//// Sequential implementation //////
-
-// the concrete state 
-val concrete_st_s : Type0
-
-// init state 
-val init_st_s : concrete_st_s
-
-// apply an operation to a state 
-val do_s (st_s:concrete_st_s) (_:op_t) : concrete_st_s
-
-// equivalence relation between the concrete states of sequential type and MRDT
-val eq_sm (st_s:concrete_st_s) (st:concrete_st) : Type0
-
-// initial states are equivalent
-val initial_eq (_:unit)
-  : Lemma (ensures eq_sm init_st_s init_st)
-
-// equivalence between states of sequential type and MRDT at every operation
-val do_eq (st_s:concrete_st_s) (st:concrete_st) (op:op_t)
-  : Lemma (requires eq_sm st_s st)
-          (ensures eq_sm (do_s st_s op) (do st op))
-
-////////////////////////////////////////////////////////////////
+          (ensures eq (merge (do l o) (do (do s1 o) o1) (do (do s2 o) o2)) (do (do (do s3 o) o1) o2)) = ()
