interface/Set_extended.fsti
@@ -8,9 +8,10 @@ val mem (#a:eqtype) (x:a) (s:t a) : bool
 val equal (#a:eqtype) (s1:t a) (s2:t a) : Type0
 val union (#a:eqtype) (s1 s2:t a) : t a
 val intersection (#a:eqtype) (s1 s2:t a) : t a
+val complement : #a:eqtype -> (s:t a) -> t a
 val difference (#a:eqtype) (s1 s2:t a) : t a
 val filter (#a:eqtype) (s:t a) (p:a -> bool) : t a
-//val remove (#a:eqtype) (s:t a) (x:a) : t a
+val remove (#a:eqtype) (s:t a) (x:a) : t a
 
 val mem_empty (#a:eqtype) (x:a)
   : Lemma (not (mem x empty))
@@ -64,6 +65,10 @@ val mem_intersection (#a:eqtype) (s1 s2:t a) (x:a)
   : Lemma (mem x (intersection s1 s2) <==> (mem x s1 /\ mem x s2))
           [SMTPat (mem x (intersection s1 s2))]
 
+val mem_complement (#a:eqtype) (s:t a) (x:a) 
+  : Lemma (mem x (complement s) = not (mem x s))
+   [SMTPat (mem x (complement s))]
+   
 val mem_difference (#a:eqtype) (s1 s2:t a) (x:a)
   : Lemma (mem x (difference s1 s2) <==> (mem x s1 /\ ~ (mem x s2)))
           [SMTPat (mem x (difference s1 s2))]
@@ -72,12 +77,12 @@ val mem_filter (#a:eqtype) (s:t a) (p:a -> bool) (x:a)
   : Lemma (mem x (filter s p) <==> (mem x s /\ p x))
           [SMTPat (mem x (filter s p))]
 
-(*val mem_remove_x (#a:eqtype) (s:t a) (x:a)
+val mem_remove_x (#a:eqtype) (s:t a) (x:a)
   : Lemma (not (mem x (remove s x)))
           [SMTPat (mem x (remove s x))]
 
 val mem_remove_y (#a:eqtype) (s:t a) (x:a) (y:a)
   : Lemma (requires x =!= y)
           (ensures mem y (remove s x) == mem y s)
-          [SMTPat (mem y (remove s x))]*)
+          [SMTPat (mem y (remove s x))]
           
