mrdts-new/Enable_wins_flag/App_new.fst
@@ -147,18 +147,18 @@ let rc_intermediate_base_left_right (l s1 s2 s3:concrete_st) (o o' o1' o1 o2:op_
         (ensures eq (merge (do l o') (do (do (do s1 o1') o') o1) (do (do (do s2 o) o') o2)) (do (do (do (do (do s3 o1') o) o') o1) o2)) = ()
 
 let rc_intermediate_2_right (l s1 s2 s3:concrete_st) (o1 o2 o o':op_t) (o_n:op_t{~ (commutes_with o_n o)})
-  : Lemma (requires distinct_ops o1 o2 /\ Fst_then_snd? (rc o1 o2) /\  
+: Lemma (requires distinct_ops o1 o2 /\ Fst_then_snd? (rc o1 o2) /\  
                     distinct_ops o o' /\ Fst_then_snd? (rc o o') /\
                     get_rid o_n <> get_rid o' (*o_n,o' must be concurrent*) /\
                     eq (merge (do l o') (do (do s1 o') o1) (do (do (do s2 o) o') o2)) (do (do (do (do s3 o) o') o1) o2))
-          (ensures eq (merge (do l o') (do (do s1 o') o1) (do (do (do (do s2 o_n) o) o') o2)) (do (do (do (do (do s3 o_n) o) o') o1) o2)) = ()
+      (ensures eq (merge (do l o') (do (do s1 o') o1) (do (do (do (do s2 o_n) o) o') o2)) (do (do (do (do (do s3 o_n) o) o') o1) o2)) = ()
 
 let rc_intermediate_2_left (l s1 s2 s3:concrete_st) (o1 o2 o o':op_t) (o_n:op_t{~ (commutes_with o_n o)})
-  : Lemma (requires distinct_ops o1 o2 /\ Fst_then_snd? (rc o1 o2) /\  
+: Lemma (requires distinct_ops o1 o2 /\ Fst_then_snd? (rc o1 o2) /\  
                     distinct_ops o o' /\ Fst_then_snd? (rc o o') /\
                     get_rid o_n <> get_rid o' (*o_n,o' must be concurrent*) /\
                     eq (merge (do l o') (do (do (do s1 o) o') o1) (do (do s2 o') o2)) (do (do (do (do s3 o) o') o1) o2))
-          (ensures eq (merge (do l o') (do (do (do (do s1 o_n) o) o') o1) (do (do s2 o') o2)) (do (do (do (do (do s3 o_n) o) o') o1) o2)) = ()
+      (ensures eq (merge (do l o') (do (do (do (do s1 o_n) o) o') o1) (do (do s2 o') o2)) (do (do (do (do (do s3 o_n) o) o') o1) o2)) = ()
 
 // In general, the events o',o_n, below should be such that these exists o, (rc o o')
 let rc_intermediate_1_v2 (l s1 s2 s3:concrete_st) (o1 o2 o' o_n:op_t)
@@ -188,36 +188,67 @@ let intermediate_base_right_one_op (l s1 s2 s3:concrete_st) (o o' o1:op_t)
                     eq (merge l (do s1 o') (do s2 o)) (do (do s3 o) o')) //***EXTRA***
           (ensures eq (merge (do l o') (do s1 o') (do (do (do s2 o) o') o1)) (do (do (do s3 o) o') o1)) = ()
 
+//orset
 let intermediate_base_right_one_op_left (l s1 s2 s3:concrete_st) (o o' o1:op_t) 
   : Lemma (requires distinct_ops o o' /\ Fst_then_snd? (rc o o') /\ distinct_ops o' o1 /\
                     eq (merge (do l o') (do (do s1 o') o1) (do s2 o')) (do (do s3 o') o1) /\
-                    (Fst_then_snd? (rc o o1) ==> eq (merge l (do s1 o1) (do s2 o)) (do (merge l s1 (do s2 o)) o1)) /\ //***EXTRA***       
-                    eq (merge l (do s1 o1) s2) (do s3 o1) /\
+                    eq (merge l (do s1 o1) s2) (do s3 o1) /\ 
+                    eq (merge (do l o') (do (do l o') o1) (do (do l o) o')) (do (do (do l o) o') o1) /\ //**EXTRA***
                     eq (merge l (do s1 o') (do s2 o)) (do (do s3 o) o')) //***EXTRA***
-          (ensures eq (merge (do l o') (do (do s1 o') o1) (do (do s2 o) o')) (do (do (do s3 o) o') o1)) = ()
+          (ensures eq (merge (do l o') (do (do s1 o') o1) (do (do s2 o) o')) (do (do (do s3 o) o') o1)) = admit()
 
+//ew flag
 let intermediate_base_left_one_op (l s1 s2 s3:concrete_st) (o o' o1:op_t) 
   : Lemma (requires distinct_ops o o' /\ Fst_then_snd? (rc o o') /\
                     eq (merge (do l o') (do s1 o') (do (do s2 o') o1)) (do (do s3 o') o1) /\
-                    (Fst_then_snd? (rc o o1) ==> eq (merge l (do s1 o1) (do s2 o)) (do (merge l s1 (do s2 o)) o1)) /\ //***EXTRA***
                     eq (merge l s1 (do s2 o1)) (do s3 o1) /\
+                    //eq (merge (do l o') (do (do l o') o1) (do (do l o) o')) (do (do (do l o) o') o1) /\ //**EXTRA***  !!CHECK
                     eq (merge l (do s1 o') (do s2 o)) (do (do s3 o) o') /\ //***EXTRA***
                     eq (merge l (do (do s1 o) o') (do s2 o')) (do (do s3 o) o')) //***EXTRA***
           (ensures eq (merge (do l o') (do (do s1 o) o') (do (do s2 o') o1)) (do (do (do s3 o) o') o1)) = ()
 
+//orset
+let intermediate_base_left_right_one_op_right1 (l s1 s2 s3:concrete_st) (o o' o1' o1:op_t) 
+  : Lemma (requires distinct_ops o o' /\ Fst_then_snd? (rc o o') /\
+                    distinct_ops o1' o' /\ Fst_then_snd? (rc o1' o') /\
+                    eq (merge (do l o') (do s1 o') (do (do s2 o') o1)) (do (do s3 o') o1) /\
+                    eq (merge (do l o') (do (do s1 o1') o') (do (do s2 o') o1)) (do (do (do s3 o1') o') o1) /\ //EXTRA
+                    eq (merge l s1 (do s2 o1)) (do s3 o1) /\
+                    eq (merge (do l o') (do (do l o') o1) (do (do l o) o')) (do (do (do l o) o') o1)) //***EXTRA***
+          (ensures eq (merge (do l o') (do (do s1 o1') o') (do (do (do s2 o) o') o1)) (do (do (do (do s3 o1') o) o') o1)) = ()
+
+//orset
+let intermediate_base_left_right_one_op_left1 (l s1 s2 s3:concrete_st) (o o' o1' o1:op_t) 
+  : Lemma (requires distinct_ops o o' /\ Fst_then_snd? (rc o o') /\
+                    distinct_ops o1' o' /\ Fst_then_snd? (rc o1' o') /\
+                    eq (merge (do l o') (do (do s1 o') o1) (do s2 o')) (do (do s3 o') o1) /\
+                    eq (merge (do l o') (do (do (do s1 o1') o') o1) (do s2 o')) (do (do (do s3 o1') o') o1) /\ //EXTRA
+                    eq (merge l (do s1 o1) s2) (do s3 o1) /\
+                    eq (merge (do l o') (do (do l o') o1) (do (do l o) o')) (do (do (do l o) o') o1)) //***EXTRA***
+          (ensures eq (merge (do l o') (do (do (do s1 o1') o') o1) (do (do s2 o) o')) (do (do (do (do s3 o1') o) o') o1)) = ()
+
+//ew flag
 let intermediate_base_left_right_one_op (l s1 s2 s3:concrete_st) (o o' o1' o1:op_t) 
   : Lemma (requires distinct_ops o o' /\ Fst_then_snd? (rc o o') /\
                     distinct_ops o1' o' /\ Fst_then_snd? (rc o1' o') /\
                     eq (merge (do l o') (do s1 o') (do (do s2 o') o1)) (do (do s3 o') o1) /\
                     eq (merge (do l o') (do (do s1 o1') o') (do (do s2 o') o1)) (do (do (do s3 o1') o') o1) /\ //EXTRA
                     eq (merge l s1 (do s2 o1)) (do s3 o1))
+                    //eq (merge (do l o') (do (do l o') o1) (do (do l o) o')) (do (do (do l o) o') o1) /\ //***EXTRA***
+                    //eq (merge (do l o') (do l o') (do (do (do l o) o') o1)) (do (do (do l o) o') o1))
           (ensures eq (merge (do l o') (do (do s1 o1') o') (do (do (do s2 o) o') o1)) (do (do (do (do s3 o1') o) o') o1)) = ()
 
-let intermediate_2_left_one_op (l s1 s2 s3:concrete_st) (o1 o o':op_t) (o_n:op_t{~ (commutes_with o_n o)})
+let intermediate_2_right_one_op (l s1 s2 s3:concrete_st) (o1 o o':op_t) (o_n:op_t{~ (commutes_with o_n o)})
   : Lemma (requires distinct_ops o o' /\ Fst_then_snd? (rc o o') /\
                     get_rid o_n <> get_rid o' (*o_n,o' must be concurrent*) /\
-                    eq (merge (do l o') (do (do s1 o) o') (do (do s2 o') o1)) (do (do (do s3 o) o') o1))
-          (ensures eq (merge (do l o') (do (do (do s1 o_n) o) o') (do (do s2 o') o1)) (do (do (do (do s3 o_n) o) o') o1)) = ()
+                    eq (merge (do l o') (do s1 o') (do (do (do s2 o) o') o1)) (do (do (do s3 o) o') o1))
+          (ensures eq (merge (do l o') (do s1 o') (do (do (do (do s2 o_n) o) o') o1)) (do (do (do (do s3 o_n) o) o') o1)) = ()
+
+let intermediate_2_left_one_op (l s1 s2 s3:concrete_st) (o1 o o':op_t) (o_n:op_t{~ (commutes_with o_n o)})
+: Lemma (requires distinct_ops o o' /\ Fst_then_snd? (rc o o') /\
+                  get_rid o_n <> get_rid o' (*o_n,o' must be concurrent*) /\
+                  eq (merge (do l o') (do (do s1 o) o') (do (do s2 o') o1)) (do (do (do s3 o) o') o1))
+      (ensures eq (merge (do l o') (do (do (do s1 o_n) o) o') (do (do s2 o') o1)) (do (do (do (do s3 o_n) o) o') o1)) = ()
 
 // In general, the events o',o_n, below should be such that these exists o, (rc o o')
 let intermediate_1_v2_one_op (l s1 s2 s3:concrete_st) (o1 o' o_n:op_t)
